\documentclass[a4paper,12p]{article}
\setcounter{tocdepth}{3}
\setcounter{secnumdepth}{3}
\usepackage[a4paper, inner=0.7cm, outer=1.7cm, top=2cm, bottom=2cm, bindingoffset=1.2cm]{geometry}
\usepackage[portuguese]{babel}
\usepackage{blindtext}
\usepackage{microtype}
\usepackage{graphicx}
\usepackage{wrapfig}
\usepackage{enumitem}
\usepackage{fancyhdr}
\usepackage{amsmath}
\usepackage{index}
\usepackage{multicol,float,listings}
\usepackage{setspace}
\usepackage[super]{nth}
\usepackage{amsmath}
\usepackage[utf8]{inputenc}
\usepackage{amssymb}
\newcommand{\dd}[1]{\mathrm{d}#1}
\makeindex

\begin{document}

	\title{\LARGE{\textbf{Resumo da Pesquisa PPGEM}}}
	\author{Luan Henrique Sirtoli}
	\date{03 de Abril de 2019}
	\maketitle

	%\tableofcontents

	%\pagenumbering{roman}
	\setcounter{page}{1}

	%\chapter{Resumo da Pesquisa PPGEM}
	\section{Fundamentos da Pesquisa}

	\begin{equation}
	H_{uq}u - G_{uu}q + \lambda W_{uq}u + \lambda S_{uu}q = \lambda^2 M_{uq}u \label{a}
	\end{equation}
	\begin{equation}
	H_{qq}u - G_{qu}q + \lambda W_{qq}u + \lambda S_{qu}q = \lambda^2 M_{qq}u
	\end{equation}
	
	A partir da equação \ref{a}
	\begin{equation}
	(H_{uq}  + \lambda W_{uq})u + (\lambda S_{uu} - G_{uu})q = \lambda^2 M_{uq}u
	\end{equation}
	\begin{equation}
	 (\lambda S_{uu} - G_{uu})q = (\lambda^2 M_{uq} - H_{uq}  - \lambda W_{uq})u
	\end{equation}
	\begin{equation}
	q = (\lambda^2 M_{uq} - H_{uq}  - \lambda W_{uq})(\lambda S_{uu} - G_{uu})^{-1}u 
	\end{equation}
	\begin{equation}
	q = (\lambda^2 M_{uq} - H_{uq}  - \lambda W_{uq})(\frac{1}{\lambda} S_{uu}^{-1} - G_{uu}^{-1})u 
	\end{equation}
	\begin{equation}
	Z = (\lambda^2 M_{uq} - H_{uq}  - \lambda W_{uq})
	\end{equation}
	\begin{equation}
	q = (Zu)(\frac{1}{\lambda} S_{uu}^{-1} - G_{uu}^{-1}) 
	\end{equation}
	
	
	
	\begin{equation}
	H_{qq}u - G_{qu}(Zu)(\frac{1}{\lambda} S_{uu}^{-1} - G_{uu}^{-1}) + \lambda W_{qq}u + \lambda S_{qu}(Zu)(\frac{1}{\lambda} S_{uu}^{-1} - G_{uu}^{-1}) = \lambda^2 M_{qq}u
	\end{equation}
	\begin{equation}
	H_{qq}u 
	- (\frac{1}{\lambda})G_{qu}S_{uu}^{-1}(Zu)
	+ G_{qu}G_{uu}^{-1}(Zu)
	+ \lambda W_{qq}u 
	+ S_{qu}S_{uu}^{-1}(Zu) 
	- \lambda S_{qu}G_{uu}^{-1}(Zu) 
	= \lambda^2 M_{qq}u
	\end{equation}
	\begin{equation}
	H_{qq}u 
	+ \lambda W_{qq}u 
	- (\frac{1}{\lambda})G_{qu}S_{uu}^{-1}(Zu)
	+ G_{qu}G_{uu}^{-1}(Zu)
	+ S_{qu}S_{uu}^{-1}(Zu) 
	- \lambda S_{qu}G_{uu}^{-1}(Zu) 
	= \lambda^2 M_{qq}u
	\end{equation}
	\begin{equation}
	H_{qq}u 
	+ \lambda W_{qq}u 
	+( - (\frac{1}{\lambda})G_{qu}S_{uu}^{-1}
	+ G_{qu}G_{uu}^{-1}
	+ S_{qu}S_{uu}^{-1}
	- \lambda S_{qu}G_{uu}^{-1})(Zu) 
	= \lambda^2 M_{qq}u
	\end{equation}
	\begin{equation}
	H_{qq}u 
	+ \lambda W_{qq}u 
	+( - (\frac{1}{\lambda})G_{qu}S_{uu}^{-1}
	+ G_{qu}G_{uu}^{-1}
	+ S_{qu}S_{uu}^{-1}
	- \lambda S_{qu}G_{uu}^{-1})
	(\lambda^2 M_{uq} - H_{uq}  - \lambda W_{uq})u 
	= \lambda^2 M_{qq}u
	\end{equation}
	\begin{equation}
	\begin{split}
	H_{qq}u 
	+ \lambda W_{qq}u 
	- (\frac{1}{\lambda}G_{qu}S_{uu}^{-1})
	(\lambda^2 M_{uq} - H_{uq}  - \lambda W_{uq})u
	+ (G_{qu}G_{uu}^{-1})
	(\lambda^2 M_{uq} - H_{uq}  - \lambda W_{uq})u \\
	+ (S_{qu}S_{uu}^{-1})
	(\lambda^2 M_{uq} - H_{uq}  - \lambda W_{uq})u
	- (\lambda S_{qu}G_{uu}^{-1})
	(\lambda^2 M_{uq} - H_{uq}  - \lambda W_{uq})u 
	= \lambda^2 M_{qq}u
	\end{split}
	\end{equation}
	
	Assumindo:
	\begin{equation}
	G_{qu}S_{uu}^{-1} = V_{qu}
	\end{equation}
	\begin{equation}
	G_{qu}G_{uu}^{-1} = T_{qu}
	\end{equation}
	\begin{equation}
	S_{qu}S_{uu}^{-1} = X_{qu}
	\end{equation}
	\begin{equation}
	S_{qu}G_{uu}^{-1} = Y_{qu}
	\end{equation}
	
	
	\begin{equation}
	\begin{split}
	H_{qq}u 
	+ \lambda W_{qq}u 
	- (\frac{1}{\lambda}V_{qu})
	(\lambda^2 M_{uq} - H_{uq}  - \lambda W_{uq})u
	+ (T_{qu})
	(\lambda^2 M_{uq} - H_{uq}  - \lambda W_{uq})u \\
	+ (X_{qu})
	(\lambda^2 M_{uq} - H_{uq}  - \lambda W_{uq})u
	- (\lambda Y_{qu})
	(\lambda^2 M_{uq} - H_{uq}  - \lambda W_{uq})u 
	= \lambda^2 M_{qq}u
	\end{split}
	\end{equation}
	\begin{equation}
	\begin{split}
	H_{qq}u 
	+ \lambda W_{qq}u 
	- (\frac{1}{\lambda})
	(\lambda^2 V_{qu}M_{uq} - V_{qu}H_{uq}  - \lambda V_{qu}W_{uq})u
	+ (\lambda^2 T_{qu}M_{uq} - T_{qu}H_{uq}  - \lambda T_{qu}W_{uq})u \\
	+ (\lambda^2 X_{qu}M_{uq} - X_{qu}H_{uq}  - \lambda X_{qu}W_{uq})u
	- (\lambda )
	(\lambda^2 Y_{qu}M_{uq} - Y_{qu}H_{uq}  - \lambda Y_{qu}W_{uq})u 
	= \lambda^2 M_{qq}u
	\end{split}
	\end{equation}
	
	\begin{gather}
	\frac{u}{\lambda} (V_{qu}H_{uq})  \\
	+ u(H_{qq} + V_{qu}W_{uq} - T_{qu}H_{uq} - X_{qu}H_{uq}) \\
	+ \lambda u (W_{qq} - V_{qu}M_{uq} - T_{qu}W_{uq} - X_{qu}W_{uq} +  Y_{qu}H_{uq})\\
	+ \lambda^2 u (T_{qu}M_{uq} + X_{qu}M_{uq} + Y_{qu}W_{uq} - M_{qq})\\
	- \lambda^3 u (Y_{qu}M_{uq})
	= 0
	\end{gather}
	
	\begin{equation}
	\begin{split}
	u(V_{qu}H_{uq})
	+ \lambda u (H_{qq} + V_{qu}W_{uq} - T_{qu}H_{uq} - X_{qu}H_{uq}) \\
	+ \lambda^2 u (W_{qq} - V_{qu}M_{uq} - T_{qu}W_{uq} - X_{qu}W_{uq} +  Y_{qu}H_{uq}) \\
	+ \lambda^3 u (T_{qu}M_{uq} + X_{qu}M_{uq} + Y_{qu}W_{uq} - M_{qq})
	- \lambda^4 u (Y_{qu}M_{uq})
	= 0
	\end{split}
	\end{equation}
	
	\begin{gather}
	A = V_{qu}H_{uq}  \\
	B = H_{qq} + V_{qu}W_{uq} - T_{qu}H_{uq} - X_{qu}H_{uq} \\
	C = W_{qq} - V_{qu}M_{uq} - T_{qu}W_{uq} - X_{qu}W_{uq} +  Y_{qu}H_{uq}\\
	D = T_{qu}M_{uq} + X_{qu}M_{uq} + Y_{qu}W_{uq} - M_{qq}\\
	E = Y_{qu}M_{uq}
	\end{gather}
	
	\begin{equation}
	\begin{split}
	u(G_{qu}S_{uu}^{-1}H_{uq})
	+ \lambda u (H_{qq} + G_{qu}S_{uu}^{-1}W_{uq} - G_{qu}G_{uu}^{-1}H_{uq} - S_{qu}S_{uu}^{-1}H_{uq})\\
	+ \lambda^2 u (W_{qq} - G_{qu}S_{uu}^{-1}M_{uq} - G_{qu}G_{uu}^{-1}W_{uq} - S_{qu}S_{uu}^{-1}W_{uq} +  S_{qu}G_{uu}^{-1}H_{uq}) \\
	+ \lambda^3 u (G_{qu}G_{uu}^{-1}M_{uq} + S_{qu}S_{uu}^{-1}M_{uq} + S_{qu}G_{uu}^{-1}W_{uq} - M_{qq}) \\
	- \lambda^4 u (S_{qu}G_{uu}^{-1}M_{uq})
	= 0
	\end{split}
	\end{equation}
	
	\begin{equation}
	uA + \lambda u B + \lambda^2 u C + \lambda^3 u D - \lambda^4 u E = 0
	\end{equation}
	
	
\end{document}
